theories/tree_test.v
@@ -125,19 +125,19 @@ Definition CutS := TA cut.
 Section Test2.
   Goal step unif emptyp fset0 empty (Or (Some OK) empty OK) = (fset0, Success, Or (Some OK) empty OK). by []. Qed.
 
-  Goal runT unif emptyp fset0 empty (Or (Some CutS) empty OK) (Some empty) None false fset0.
+  Goal runT unif emptyp fset0 empty (Or (Some CutS) empty OK) (Some (empty, None)) false fset0.
     apply: StepT => //=.
     apply: StopT => //.
   Qed.
 
   Goal forall r, 
-    runT unif emptyp fset0 empty (Or (Some CutS) empty r) (Some empty) None false fset0.
+    runT unif emptyp fset0 empty (Or (Some CutS) empty r) (Some (empty, None)) false fset0.
     move=> r.
     apply: StepT => //.
     apply: StopT => //=.
   Qed.
 
-  Goal runT unif emptyp fset0 empty (Or (Some OK) empty (Or (Some OK) empty OK)) (Some empty) (Some (Or None empty (((Or (Some OK) empty OK))))) false fset0.
+  Goal runT unif emptyp fset0 empty (Or (Some OK) empty (Or (Some OK) empty OK)) (Some (empty, (Some (Or None empty (((Or (Some OK) empty OK))))))) false fset0.
   Proof. apply: StopT => //=. Qed.
 
   (* (Dead \/ !) \/ C *)
